src/Crypto/src/WrappedHKDF.dfy
@@ -3,6 +3,7 @@
 
 include "HKDF/HKDF.dfy"
 include "HKDF/HMAC.dfy"
+include "Digest.dfy"
 include "../Model/AwsCryptographyPrimitivesTypes.dfy"
 
 /*
@@ -11,27 +12,64 @@ include "../Model/AwsCryptographyPrimitivesTypes.dfy"
 module WrappedHKDF {
   import opened Wrappers
   import opened UInt = StandardLibrary.UInt
+  import StandardLibrary
   import Types = AwsCryptographyPrimitivesTypes
   import HMAC
   import HKDF
+  import Digest
 
-  method Extract(input: Types.HkdfExtractInput) returns (prk: seq<uint8>)
+  method Extract(input: Types.HkdfExtractInput)
+    returns (prk: seq<uint8>)
+    requires (input.salt.None? || |input.salt.value| != 0)
+    requires (|input.ikm| < INT32_MAX_LIMIT)
   {
-    var HkdfExtractInput(digest, salt, ikm) := input;
+    var HkdfExtractInput(digestAlgorithm, salt, ikm) := input;
+
+    var hmac := new HMAC.HMac(digestAlgorithm);
+    prk := HKDF.Extract(
+      hmac,
+      salt.UnwrapOr(StandardLibrary.Fill(0, Digest.Length(digestAlgorithm))),
+      ikm,
+      digestAlgorithm
+    );
   }
 
-  method Expand(input: Types.HkdfExpandInput) returns (okm: seq<uint8>)
+  method Expand(input: Types.HkdfExpandInput)
+    returns (okm: seq<uint8>)
+    requires 1 <= input.expectedLength as int <= 255 * Digest.Length(input.digestAlgorithm)
+    requires |input.info| < INT32_MAX_LIMIT
+    requires Digest.Length(input.digestAlgorithm) == |input.prk|
   {
-    var HkdfExpandInput(digest, prk, info, expectedLength) := input;
+    var HkdfExpandInput(digestAlgorithm, prk, info, expectedLength) := input;
+
+    var hmac := new HMAC.HMac(digestAlgorithm);
+    var output, _ := HKDF.Expand(
+      hmac,
+      prk,
+      info,
+      expectedLength as int,
+      digestAlgorithm
+    );
   }
 
   /*
    * The RFC 5869 KDF. Outputs L bytes of output key material.
    */
-  method Hkdf(input: Types.HkdfInput) returns (okm: seq<uint8>)
+  method Hkdf(input: Types.HkdfInput)
+    returns (okm: seq<uint8>)
+    requires 0 <= input.expectedLength as int <= 255 * Digest.Length(input.digestAlgorithm)
+    requires (input.salt.None? || |input.salt.value| != 0)
+    requires |input.info| < INT32_MAX_LIMIT
+    requires |input.ikm| < INT32_MAX_LIMIT
   {
     var HkdfInput(digest, salt, ikm, info, expectedLength) := input;
 
-    // okm := HKDF.Hkdf(digest, salt, ikm, info, expectedLength);
+    okm := HKDF.Hkdf(
+      digest,
+      salt,
+      ikm,
+      info,
+      expectedLength as int
+    );
   }
 }
